\documentclass{article}
\usepackage{amsmath}
\usepackage{forest}
\usepackage{tikz,pgf}
\usepackage{fancyhdr}
\pagestyle{fancy}
\fancyhf{}
\fancyhead[L]{CS3230 - Assignment 1}
\fancyhead[R]{Daniel Alfred (A0184588J)}
\fancyfoot[C]{\thepage}
\begin{document}
	\begin{enumerate}
		\item{
			\begin{align*}
			&g_{1}(n) = \Theta(n!)\\
			&g_{2}(n) = \Theta(n^3\lg n)\\
			&g_{3}(n) = \Theta(n^{\lg n})\\
			&g_{4}(n) = \Theta(\sqrt{n})\\
			&g_{5}(n) = \Theta(2^{\lg n})\\
			&g_{6}(n) = \Theta(\lg ^3n)\\
			&g_{7}(n) = \Theta(2 ^ n)\\
			&g_{8}(n) = \Theta(n^3\lg\lg n)\\
			g_6 << g_4 << g_5 <&< g_8 << g_2 << g_3 << g_7 << g_1
			\end{align*}
		}
		\pagebreak
		\item{
			\begin{enumerate}
				\item {
					\begin{align*}
					T(n) &= 4\cdot T(n/2) + \Theta(n^2\lg^3 n)\\
					a &= 4\\
					b &= 2\\
					f(n) &= \Theta(n^2\lg^3n)\\
					n^{\log_ba} &= n^{\log_24}\\
					&= n^2\\
					Case2:\\
					f(n) &= \Theta(n^{log_24} \lg^1 n)\\
					T(n) &= \Theta(n^2\lg^2 n)
					\end{align*}
				}
				\item{
					\begin{align*}
						T(n) &= 3\cdot T(n/2) + 5n\\
						&\begin{forest}
							[$T(n) + 5n$
								[$T(n/2) + \frac{5n}{2}$
									[... [1]]
									[... [1]]
									[... [1]]
								] 
								[$T(n/2) + \frac{5n}{2}$
									[... [1]]
									[... [1]]
									[... [1]]
								] 
								[$T(n/2) + \frac{5n}{2}$
									[... [1]]
									[... [1]]
									[... [1]]
								]
							]
						\end{forest}\\
						T(n) &= 1\cdot3^{\lg n} + 5n + \frac{3}{2}^1 5n + \frac{3}{2}^2 5n + \dots\\
						T(n) &= 3^{\lg n} + 5n\cdot\sum_{i = 0}^{\lg n - 1}\frac{3}{2}^i\\
						T(n) &= ((2^{\lg 3})^{\lg n})+5n\cdot\frac{\frac{3}{2}^{\lg n} - 1}{\frac{3}{2} - 1}\\
						T(n) &= 2^{\lg n \cdot \lg 3} + 10n \cdot (\frac{3^{\lg n}}{2^{\lg n}} - 1)\\
						T(n) &= n^{\lg 3} + 10n \cdot (\frac{n ^{\lg 3}}{n} - 1)\\
						T(n) &= 11 n^{\lg 3} - 10n\\
						T(n) &= O(n^{\lg 3})
					\end{align*}
				}
				\pagebreak
				\item{
					\begin{align*}
						U(n)&=\frac{2}{n-1}\sum_{k=1}^{n-1}U(k) + 5n\\
						&=\frac{2}{n-1}U(n-1) + 10 + \frac{2}{n-1}\sum_{k=1}^{n-2}U(k) + 5(n-2)\\
						&=\frac{2}{n-1}U(n-1) + \frac{n-2}{n-1}U(n-1) + 10\\
						&=(\frac{2}{n-1} + \frac{n-2}{n-1})U(n-1) + 10\\
						U(n+1)&=(\frac{2}{n} + \frac{n-1}{n})U(n) + 10\\
						&=(\frac{n+1}{n})U(n) + 10\\
						&=(\frac{n+1}{n})((\frac{n}{n-1})U(n-1) +10)+10\\
						&=n + 1 + 10(1 + \frac{n+1}{n}+\frac{n+1}{n-1}+\dots+\frac{n+1}{1})\\
						&=n+1+10(1+(n+1)*\sum_{x=1}^{n}\frac{1}{x})\\
						&=n+1+10(1+(n+1)*\ln n)\\
						&=n+1 + 10 + 10n\ln n + 10\ln n\\
						&=O(n \log n)
					\end{align*}
				}
			\end{enumerate}
		}
		\pagebreak
		\item {
			\begin{enumerate}
				\item {
					\begin{align*}
						f(n) &\leq O(g(n)) < o(g(n))\\
						f(n) &\leq k n^{c-\epsilon} < k'n^c\\
						\text{Proving }kn^{c-\epsilon} &< k'n^c:\\
						\lim_{n\to\infty}\frac{n^c}{n^{c-\epsilon}}&=\lim_{n\to\infty}n^\epsilon\to\infty\\
						\infty &> \frac{k}{k'} \text{ because k \& k' is finite}\\
						&\text{Proven}
					\end{align*}
				}
				\item {
					\begin{align*}
						\text{let }f(n) &= \frac{n^c}{\lg n}\\
						f(n) \in o(g(n)) &\iff \lim_{n\to\infty}\frac{f(n)}{g(n)} = 0\\
						\lim_{n\to\infty}\frac{f(n)}{g(n)} &=\lim_{n\to\infty}\frac{\frac{n^c}{\lg n}}{n^c}\\
						&=\lim_{n\to\infty}\frac{1}{\lg n} \to 0\\
						\\
						f(n) \in O(g(n)) &\iff \lim_{n\to\infty}\frac{f(n)}{g(n)} < \infty\\
						\lim_{n\to\infty} \frac{f(n)}{g(n)} &= \lim_{n\to\infty}\frac{\frac{n^c}{\lg n}}{n^{c-\epsilon}}\\
						&=\lim_{n\to\infty}\frac{\frac{1}{\lg n}}{n^{-\epsilon}}\\
						&=\lim_{n\to\infty}\frac{n^\epsilon}{\lg n}\\
						&=\lim_{n\to\infty}\frac{\epsilon n^{\epsilon-1}}{\frac{1}{n}} \text{ (L'Hopital)}\\
						&=\lim_{n\to\infty}\epsilon n^\epsilon \to \infty\\
						f(n) &\notin O(g(n))\\
						&\text{Disproven}
					\end{align*}
				}
			\end{enumerate}
		}
	\end{enumerate}
\end{document}